theories/Core/Semantic/Evaluation/Lemmas.v
@@ -6,6 +6,18 @@ From Mctt.Core.Semantic.Evaluation Require Import Definitions.
 Import Domain_Notations.
 
 Section functional_eval.
+  Lemma functional_fst_app : 
+    (forall a r1,
+      {{ π₁ a ↘ r1 }} ->
+        forall r2,
+        {{ π₁ a ↘ r2 }} ->
+        r1 = r2).
+  Proof.
+    intros. 
+    inversion_by_head fst_app; subst; 
+    progressive_inversion; reflexivity.
+  Qed.
+
   Lemma functional_eval :
     (forall M ρ m1,
         {{ ⟦ M ⟧ ρ ↘ m1 }} ->
@@ -22,6 +34,11 @@ Section functional_eval.
           forall r2,
             {{ $| m & n |↘ r2 }} ->
             r1 = r2) /\
+      (forall a r1,
+          {{ π₂ a ↘ r1 }} ->
+            forall r2,
+              {{ π₂ a ↘ r2 }} ->
+              r1 = r2) /\
       (forall a B BR m1 m2 n ρ r1,
           {{ eqrec n as Eq a m1 m2 ⟦return B | refl -> BR end⟧ ρ ↘ r1 }} ->
           forall r2,
@@ -32,10 +49,10 @@ Section functional_eval.
           forall ρσ2,
             {{ ⟦ σ ⟧s ρ ↘ ρσ2 }} ->
             ρσ1 = ρσ2).
-  Proof with ((on_all_hyp: fun H => erewrite H in *; eauto); solve [eauto]) using.
+  Proof with ((on_all_hyp: fun H => erewrite H in *; eauto); solve [eauto using functional_fst_app]) using.
     apply eval_mut_ind; intros;
-      try progressive_inversion;
-       try do 2 f_equal; try reflexivity.
+       progressive_inversion; 
+       try do 2 f_equal; try reflexivity...
   Qed.
 
   Corollary functional_eval_exp : forall M ρ m1 m2,
@@ -62,6 +79,14 @@ Section functional_eval.
     pose proof functional_eval; intuition.
   Qed.
 
+  Corollary functional_snd_app : forall m r1 r2,
+      {{ π₂ m ↘ r1 }} ->
+      {{ π₂ m ↘ r2 }} ->
+      r1 = r2.
+  Proof.
+    pose proof functional_eval; intuition; eauto.
+  Qed.
+
   Corollary functional_eval_eqrec : forall a B BR m1 m2 n ρ r1 r2,
       {{ eqrec n as Eq a m1 m2 ⟦return B | refl -> BR end⟧ ρ ↘ r1 }} ->
       {{ eqrec n as Eq a m1 m2 ⟦return B | refl -> BR end⟧ ρ ↘ r2 }} ->
@@ -80,7 +105,7 @@ Section functional_eval.
 End functional_eval.
 
 #[export]
-Hint Resolve functional_eval_exp functional_eval_natrec functional_eval_app functional_eval_eqrec functional_eval_sub : mctt.
+Hint Resolve functional_eval_exp functional_eval_natrec functional_eval_app functional_fst_app functional_snd_app functional_eval_eqrec functional_eval_sub : mctt.
 
 Ltac functional_eval_rewrite_clear1 :=
   let tactic_error o1 o2 := fail 3 "functional_eval equality between" o1 "and" o2 "cannot be solved by mauto" in
@@ -90,6 +115,12 @@ Ltac functional_eval_rewrite_clear1 :=
       clean replace m2 with m1 by first [solve [mauto 2] | tactic_error m2 m1]; clear H2
   | H1 : {{ $| ^?m & ^?n |↘ ^?r1 }},
       H2 : {{ $| ^?m & ^?n |↘ ^?r2 }} |- _ =>
+      clean replace r2 with r1 by first [solve [mauto 2] | tactic_error r2 r1]; clear H2
+  | H1 : {{ π₁ ^?m ↘ ^?r1 }},
+      H2 : {{ π₁ ^?m ↘ ^?r2 }} |- _ =>
+      clean replace r2 with r1 by first [solve [mauto 2] | tactic_error r2 r1]; clear H2
+  | H1 : {{ π₂ ^?m ↘ ^?r1 }},
+      H2 : {{ π₂ ^?m ↘ ^?r2 }} |- _ =>
       clean replace r2 with r1 by first [solve [mauto 2] | tactic_error r2 r1]; clear H2
   | H1 : {{ rec ^?m ⟦return ^?A | zero -> ^?MZ | succ -> ^?MS end⟧ ^?ρ ↘ ^?r1 }},
       H2 : {{ rec ^?m ⟦return ^?A | zero -> ^?MZ | succ -> ^?MS end⟧ ^?ρ ↘ ^?r2 }} |- _ =>
